Challenge/Ripemd160/Submission/Proofs/Bytecode/GuardInstructionWindow.lean
@@ -60,13 +60,8 @@ def tail : List Instr :=
   op 0x9a,
   op 0x8c,
   op 0x8c,
-  op 0x10,
-  .push 2 600,
-  op 0x57,
-  op 0x8b,
-  op 0x36,
-  op 0x14,
-  .push 2 415,
+  op 0x18,
+  .push 2 599,
   op 0x57,
   op 0x50,
   op 0x50,
@@ -119,7 +114,7 @@ def tail : List Instr :=
   op 0x1a,
   .push 1 7,
   op 0x18,
-  .push 2 5188,
+  .push 2 5149,
   op 0x57,
   .push 17 342276208914615837337402008677671501826,
   op 0x36,
@@ -173,7 +168,7 @@ def tail : List Instr :=
 ]
 theorem tail_eq : Artifact.submissionArtifact.instructions.drop 3756 = tail := by rfl
 
-theorem pc_base : Artifact.submissionArtifact.instructionPC 3756 = 4689 := by
+theorem pc_base : Artifact.submissionArtifact.instructionPC 3756 = 4657 := by
   rw [instructionPC_eq_byteLength]
   rfl
 
@@ -183,7 +178,7 @@ theorem get (index : Nat) :
 
 theorem pc (index : Nat) :
     Artifact.submissionArtifact.instructionPC (3756 + index) =
-      4689 + byteLength (tail.take index) := by
+      4657 + byteLength (tail.take index) := by
   rw [InstructionWindow.pc_drop, pc_base, tail_eq]
 
 #print axioms get
